dh_auth/initiator.v
@@ -1,0 +1,207 @@
+From stdpp Require Import base gmap.
+From mathcomp Require Import ssreflect.
+From mathcomp Require ssrbool.
+From iris.algebra Require Import agree auth csum gset gmap excl frac.
+From iris.algebra Require Import reservation_map.
+From iris.heap_lang Require Import notation proofmode.
+From cryptis Require Import lib term gmeta nown cryptis primitives tactics.
+From cryptis Require Import role.
+From cryptis.dh_auth Require Import shared.
+
+Set Implicit Arguments.
+Unset Strict Implicit.
+Unset Printing Implicit Defensive.
+
+Section Verif.
+
+Context `{!heapGS Σ, !cryptisGS Σ}.
+Notation iProp := (iProp Σ).
+
+Implicit Types (rl : role) (t kI kR nI nR sI sR kS : term).
+Implicit Types (γ γa γb : gname) (ok : bool).
+Implicit Types (ts : nat) (T : gset term).
+Implicit Types (si : sess_info).
+
+Variable N : namespace.
+
+Definition initiator : val := λ: "c" "vkI" "skI" "vkR",
+  let: "a"    := mknonce #() in
+  let: "ga"   := mkkeyshare "a" in
+  let: "m1"   := term_of_list ["ga"; "vkI"] in
+  send "c" "m1";;
+  bind: "m2"   := tdec (N.@"m2") "vkR" (recv "c") in
+  bind: "m2"   := list_of_term "m2" in
+  list_match: ["ga'"; "gb"; "vkI'"] := "m2" in
+  assert: eq_term "ga" "ga'" && eq_term "vkI" "vkI'" in
+  let: "gab" := texp "gb" "a" in
+  let: "secret" := term_of_list ["ga"; "gb"; "gab"] in
+  let: "kS" := tag (nroot.@"keys".@"sym") "secret" in
+  let: "m3" := tenc (N.@"m3") "skI" (term_of_list ["ga"; "gb"; "vkR"]) in
+  send "c" "m3";;
+  SOME (mkskey "kS").
+
+Ltac protocol_failure :=
+  by intros; wp_pures; iApply ("Hpost" $! None); iFrame.
+
+Lemma wp_initiator c kI kR dq n T E :
+  ↑cryptisN ⊆ E →
+  channel c -∗
+  cryptis_ctx -∗
+  dh_auth_ctx N -∗
+  public (TKey Dec kI) -∗
+  public (TKey Dec kR) -∗
+  {{{ ●H{dq|n} T }}}
+    initiator c (TKey Dec kI) (TKey Enc kI) (TKey Dec kR) @ E
+  {{{ okS, RET (repr (Spec.mkskey <$> okS));
+      ●H{dq|n} T ∗
+      if okS is Some kS then
+        let si := SessInfo kI kR kS n T in
+        minted kS ∗
+        □ (∀ kt, public (TKey kt kS) ↔ ▷ session_fail si) ∗
+        (session_fail si ∨ session si ∗ term_token kS (↑nroot.@"client"))
+      else True
+ }}}.
+Proof.
+rewrite /initiator.
+iIntros (?) "#chan_c #ctx #(? & ?) #p_kI #p_kR %Ψ !> hon Hpost".
+iMod (minted_at_list with "[//] hon") as "[hon list]" => //;
+  try solve_ndisj.
+wp_pures.
+iDestruct "list" as "(%M & #m_M & #minted_at_M)".
+wp_bind (mknonce _).
+iApply (wp_mknonce_freshN M
+          (λ _, public_at n (TKey Enc kI) ∨
+                public_at n (TKey Enc kR))%I
+          dh_auth_pred
+          (λ a, {[TExp (TInt 0) [a]]})) => //.
+- iIntros "% ?". rewrite big_sepS_forall. by iApply "m_M".
+- iIntros "%a". rewrite big_sepS_singleton minted_TExp minted_TInt /=.
+  iIntros "!>"; iSplit; eauto.
+  by iIntros "(_ & ? & _)".
+iIntros "%a %fresh #m_a #p_a #a_pred token".
+rewrite big_sepS_singleton.
+iPoseProof (honest_auth_frag with "hon") as "#honI".
+wp_pures. wp_bind (mkkeyshare _). iApply wp_mkkeyshare => //.
+iIntros "!> _". wp_pures. wp_list. wp_term_of_list.
+wp_pure _ credit:"H1".
+wp_pure _ credit:"H2".
+iAssert (public (TExp (TInt 0) [a])) as "p_ga".
+{ iApply public_TExp1.
+  rewrite minted_TInt. do 2![iSplit => //].
+  iRight. iApply "a_pred". iModIntro. iModIntro.
+  iIntros "%g %ks %e".
+  case/TExp_inj: e => _ perm.
+  by rewrite -(Permutation_length perm). }
+wp_bind (send _ _). iApply wp_send => //.
+{ rewrite public_of_list /=. iModIntro.
+  do 2?[iSplit => //]. }
+wp_pure _ credit:"H3".
+wp_pures. wp_bind (recv _). iApply wp_recv => //.
+iIntros "%m2 #p_m2". wp_tdec m2; last by protocol_failure.
+wp_pures. wp_list_of_term m2; last by protocol_failure.
+wp_pures. wp_list_match => [ga' gb vkI' -> {m2}|]; last by protocol_failure.
+wp_eq_term e; last by protocol_failure. subst ga'.
+wp_pures. wp_eq_term e; last by protocol_failure. subst vkI'.
+iAssert (public gb)%I as "#p_gb".
+{ iPoseProof (public_TEncE with "p_m2 [//]") as "[p|p]".
+  - rewrite public_of_list /=.
+    by iDestruct "p" as "(_ & _ & ? & _)".
+  - iDestruct "p" as "(_ & _ & #p)".
+    iSpecialize ("p" with "p_kR").
+    rewrite public_of_list /=.
+    by iDestruct "p" as "(_ & ? & ? & _)". }
+iPoseProof (public_minted with "p_m2") as "m_m2".
+rewrite minted_TEnc minted_tag minted_of_list /=.
+iDestruct "m_m2" as "(_ & _ & m_gb & _)".
+wp_pures. wp_bind (texp _ _). iApply wp_texp.
+wp_pures. wp_list. wp_term_of_list. wp_pures.
+set secret := Spec.of_list [TExp (TInt 0) [a]; gb; Spec.texp gb a].
+wp_tag.
+set kS := Spec.tag (nroot.@"keys".@"sym") _. wp_pures.
+wp_pures. wp_list. wp_term_of_list. wp_tenc.
+iAssert ( |={E}=>
+    ●H{dq|n} T ∗
+    (public_at n (TKey Enc kR) ∧ ⌜TKey Enc kR ∉ T⌝ ∨
+    ∃ b,
+     ⌜gb = TExp (TInt 0) [b]⌝ ∗
+     □ (public b ↔ ▷ □ (public_at n (TKey Enc kI) ∨
+                        public_at n (TKey Enc kR))) ∗
+     term_meta kS (nroot.@"info") (kI, kR, n) ∗
+     term_token kS (↑nroot.@"client")))%I
+  with "[hon token H3]"
+  as "{p_m2} > (hon & p_m2)".
+{ iPoseProof (public_TEncE with "p_m2 [//]") as "{p_m2} p_m2".
+  iDestruct "p_m2" as "[[comp _]  | (#i_m2 & _ & _)]".
+  { iMod (public_atI with "[ctx] [H3] [hon] [comp]")
+      as "[hon #comp']" => //; try solve_ndisj.
+    iPoseProof (honest_frag_public_at with "honI comp'") as "%" => //.
+    iFrame. eauto. }
+  iMod (lc_fupd_elim_later_pers with "H3 i_m2") as "{i_m2} #i_m2".
+  iDestruct "i_m2"
+    as "(%ga & %b & %kI' & %n' & %T' & %e_m2 &
+         m_ga & ? & _ & honR & escrow & pred_b)".
+  case/Spec.of_list_inj: e_m2 => <- -> <- {ga gb kI'} in secret kS *.
+  iPoseProof (honest_auth_frag_agree with "hon honR") as "[% %]".
+  case: (decide (n' < n)) => [contra|?].
+  { iPoseProof ("minted_at_M" with "[//] m_ga") as "%ga_M".
+    move/(_ _ ga_M)/subtermsP: fresh.
+    rewrite subterms_TExp /= !elem_of_union => fresh.
+    case: fresh.
+    right. right. left. apply/subtermsP. apply/STRefl. }
+  have ? : n' = n by lia. subst n'.
+  iPoseProof (honest_frag_agree with "honR honI") as "->".
+  iMod (escrowE with "escrow token") as ">token" => //.
+  rewrite /kS /secret !Spec.texpA TExpC2. iFrame.
+  iModIntro. iRight. iExists b. by do !iSplit => //.
+}
+set m3 := Spec.tenc _ _ _.
+iAssert (public m3) as "#p_m3".
+{ iApply (public_TEncIS with "[] [//] [#]") => //.
+  - by rewrite !public_minted !minted_TKey.
+  - iExists a, gb, kR, n, T. do 4![iSplitR => //].
+    iDestruct "p_m2" as "[[#? _]|p_m2]"; eauto.
+    iDestruct "p_m2" as "(%b & % & #? & #? & _)".
+    iRight. by eauto.
+  - rewrite minted_of_list /= minted_TExp /= minted_TInt minted_TKey.
+    rewrite !public_minted !minted_TKey. by do ![iSplitL => //].
+  - iIntros "!> _".
+    rewrite public_of_list /=.
+    by do ![iSplit => //]. }
+wp_pures. wp_bind (send _ _). iApply wp_send => //.
+wp_pures. wp_bind (mkskey _). iApply wp_mkskey.
+pose si := SessInfo kI kR kS n T.
+iAssert (minted kS) as "#?".
+{ rewrite minted_tag minted_of_list /= minted_TExp /= minted_TInt.
+  do !iSplit => //.
+  iApply minted_texp => //. }
+iAssert (□ (∀ kt, public (TKey kt kS) ↔ ▷ session_fail si))%I as "#sec_sk".
+{ iIntros "%kt". iSplitL; last first.
+  { iIntros "!> #comp".
+    rewrite (public_TKey kt) public_tag. iLeft.
+    rewrite public_of_list /=. do !iSplit => //.
+    iApply public_texp => //.
+    iApply "p_a". eauto. }
+  iDestruct "p_m2" as "[[#? %comp]|p_m2]".
+  { iIntros "!> _ !>". by iRight. }
+  iDestruct "p_m2" as "(%b & -> & #p_b & #p_m2 & _)".
+  iIntros "!> #p_sk".
+  iPoseProof (public_sym_keyE with "[//] p_sk") as "{p_sk} >p_sk".
+  rewrite Spec.texpA in secret kS si *.
+  rewrite /secret public_of_list /= public_TExp2.
+  iDestruct "p_sk" as "(_ & _ & p_sk & _)".
+  iDestruct "p_sk" as "[[_ #p_b'] | [[_ p_a'] | (_ & a_pred' & _)]]".
+  + iPoseProof ("p_b" with "p_b'") as "{p_b} p_b". by eauto.
+  + iPoseProof ("p_a" with "p_a'") as "hon'". by eauto.
+  + iPoseProof ("a_pred" with "a_pred'") as ">%contra".
+    by have := contra _ _ eq_refl. }
+wp_pures. iApply ("Hpost" $! (Some kS)). iFrame.
+rewrite -[SessInfo _ _ _ _ _]/si.
+iSplitR => //.
+iSplitR => //.
+iDestruct "p_m2" as "[[#fail _]|p_m2]".
+{ iLeft. by iRight. }
+iDestruct "p_m2" as "(%b & -> & #p_b & #p_m2 & token)".
+iRight. iFrame. iModIntro. by iSplit.
+Qed.
+
+End Verif.
