dh_auth/responder.v
@@ -1,0 +1,222 @@
+From stdpp Require Import base gmap.
+From mathcomp Require Import ssreflect.
+From mathcomp Require ssrbool.
+From iris.algebra Require Import agree auth csum gset gmap excl frac.
+From iris.algebra Require Import reservation_map.
+From iris.heap_lang Require Import notation proofmode.
+From cryptis Require Import lib term gmeta nown cryptis primitives tactics.
+From cryptis Require Import role.
+From cryptis.dh_auth Require Import shared.
+
+Set Implicit Arguments.
+Unset Strict Implicit.
+Unset Printing Implicit Defensive.
+
+Section Verif.
+
+Context `{!heapGS Σ, !cryptisGS Σ}.
+Notation iProp := (iProp Σ).
+
+Implicit Types (rl : role) (t kI kR nI nR sI sR kS : term).
+Implicit Types (γ γa γb : gname) (ok : bool).
+Implicit Types (ts : nat) (T : gset term).
+Implicit Types (si : sess_info).
+
+Variable N : namespace.
+
+Definition responder : val := λ: "c" "vkR" "skR",
+  let: "m1" := recv "c" in
+  bind: "m1" := list_of_term "m1" in
+  list_match: ["ga"; "vkI"] := "m1" in
+  bind: "kt" := is_key "vkI" in
+  assert: "kt" = repr Dec in
+  let: "b" := mknonce #() in
+  let: "gb" := mkkeyshare "b" in
+  let: "m2" := tenc (N.@"m2") "skR" (term_of_list ["ga"; "gb"; "vkI"]) in
+  send "c" "m2";;
+  bind: "m3" := tdec (N.@"m3") "vkI" (recv "c") in
+  bind: "m3" := list_of_term "m3" in
+  list_match: ["ga'"; "gb'"; "vkR'"] := "m3" in
+  assert: eq_term "ga" "ga'" && eq_term "gb" "gb'" && eq_term "vkR" "vkR'" in
+  let: "gab" := texp "ga" "b" in
+  let: "secret" := term_of_list ["ga"; "gb"; "gab"] in
+  let: "kS" := tag (nroot.@"keys".@"sym") "secret" in
+  SOME ("vkI", mkskey "kS").
+
+Ltac protocol_failure :=
+  by intros; wp_pures; iApply ("Hpost" $! None); iFrame.
+
+Lemma wp_responder c kR dq n T E :
+  ↑cryptisN ⊆ E →
+  channel c -∗
+  cryptis_ctx -∗
+  dh_auth_ctx N -∗
+  public (TKey Dec kR) -∗
+  {{{ ●H{dq|n} T }}}
+    responder c (TKey Dec kR) (TKey Enc kR) @ E
+  {{{ okS,
+      RET (repr ((λ p, pair p.1 (Spec.mkskey p.2)) <$> okS));
+      ●H{dq|n} T ∗
+      if okS is Some (vkI, kS) then ∃ kI,
+        let si := SessInfo kI kR kS n T in
+        ⌜vkI = TKey Dec kI⌝ ∗
+        public vkI ∗
+        minted kS ∗
+        □ (∀ kt, public (TKey kt kS) ↔ ▷ session_fail si) ∗
+        session si ∗
+        term_token kS (↑nroot.@"server")
+      else True
+ }}}.
+Proof.
+iIntros "% #chan_c #? (#? & #?) #p_vkR !> %Φ hon_auth Hpost".
+wp_lam. wp_pures. wp_bind (recv _). iApply wp_recv => //.
+iIntros "%m1 #p_m1". wp_pures.
+wp_list_of_term m1; last by protocol_failure.
+wp_pures. wp_list_match => [ga vkI -> {m1}|]; last by protocol_failure.
+rewrite public_of_list /=.
+iDestruct "p_m1" as "(p_ga & p_vkI & _)".
+iPoseProof (public_minted with "p_ga") as "m_ga".
+iMod (minted_atI with "[//] hon_auth m_ga")
+  as "[hon_auth #ma_ga]"; first by solve_ndisj.
+wp_bind (is_key _). iApply wp_is_key.
+case: Spec.is_keyP => [kt kI -> {vkI}|]; last by protocol_failure.
+wp_pures. case: kt => //=; first by protocol_failure.
+wp_pures. wp_bind (mknonce _).
+iApply (wp_mknonce_freshN ∅
+          (λ _, public_at n (TKey Enc kI) ∨
+                public_at n (TKey Enc kR))%I
+          dh_auth_pred
+          (λ b, {[Spec.tag (nroot.@"keys".@"sym")
+                    (Spec.of_list [ga; TExp (TInt 0) [b]; Spec.texp ga b])]}))
+       => //.
+- iIntros "%". rewrite elem_of_empty. iIntros "[]".
+- iIntros "%b".
+  rewrite big_sepS_singleton minted_tag minted_of_list /=.
+  rewrite minted_TExp minted_TInt /=.
+  iModIntro. iSplit.
+  + iIntros "#?". do !iSplit => //.
+    by iApply minted_texp => //.
+  + by iIntros "(_ & (_ & ? & _) & _)".
+iIntros "%b _ #m_b #p_b #dh_gb token".
+rewrite big_sepS_singleton.
+set gb := TExp (TInt 0) [b].
+set gab := Spec.texp ga b.
+set kS := Spec.tag _ _.
+rewrite (term_token_difference _ (↑nroot.@"client")) //.
+iDestruct "token" as "[client token]".
+iMod (escrowI cryptisN _ (term_token ga ⊤) (term_token kS (↑nroot.@"client"))
+       with "client []") as "#client".
+{ iExists (term_meta ga nroot ()). iSplit.
+  - iIntros "!> [token #meta]".
+    by iDestruct (term_meta_token with "token meta") as "[]".
+  - iIntros "!> token".
+    by iMod (term_meta_set nroot () with "token") as "#meta". }
+rewrite (term_token_difference _ (↑nroot.@"server") (_ ∖ _)); last solve_ndisj.
+iDestruct "token" as "[server token]".
+iMod (term_meta_set (nroot.@"info") (kI, kR, n) with "token") as "#info".
+  solve_ndisj.
+iAssert (public gb) as "#p_gb".
+{ iApply public_TExp1. rewrite minted_TInt.
+  do ![iSplit => //].
+  iRight. iApply "dh_gb". iIntros "!> !> %g %ts %e".
+  case/TExp_inj: e => _ perm.
+  by rewrite -(Permutation_length perm). }
+wp_pure _ credit:"H1".
+wp_pure _ credit:"H2".
+wp_bind (mkkeyshare _). iApply wp_mkkeyshare => //.
+iIntros "!> _". wp_pures. wp_list. wp_term_of_list. wp_tenc.
+iPoseProof (honest_auth_frag with "hon_auth") as "#honR".
+wp_pures. wp_bind (send _ _). iApply wp_send => //.
+{ iModIntro.
+  iApply public_TEncIS => //.
+  - by rewrite public_minted !minted_TKey.
+  - iModIntro.
+    iExists ga, b, kI, n, T.  by do ![iSplitL => //].
+  - rewrite minted_of_list /= minted_TExp minted_TInt /=.
+    rewrite !public_minted !minted_TKey. by do ![iSplitL => //].
+  - iIntros "!> _". rewrite public_of_list /=.
+    by eauto. }
+wp_pures. wp_bind (recv _). iApply wp_recv => //.
+iIntros "%m3 #p_m3".
+wp_tdec m3; last by protocol_failure.
+wp_pures. wp_list_of_term m3; last by protocol_failure.
+wp_list_match => [ga' gb' vkR' -> {m3}|]; last by protocol_failure.
+wp_eq_term e; last by protocol_failure. subst ga'.
+wp_eq_term e; last by protocol_failure. subst gb'.
+wp_eq_term e; last by protocol_failure. subst vkR'.
+wp_pure _ credit:"H3".
+wp_bind (texp _ _). iApply wp_texp.
+wp_pure _ credit:"H4".
+iPoseProof (public_TEncE with "p_m3 [//]") as "{p_m3} p_m3".
+rewrite public_of_list /=.
+wp_pures. wp_list. wp_term_of_list.
+wp_pures. wp_tag. rewrite -/kS. pose si := SessInfo kI kR kS n T.
+iAssert ( |={E}=> ●H{dq|n} T ∗
+  □ (session_fail si ∧
+  ⌜¬ (TKey Enc kI ∈ T ∧ TKey Enc kR ∈ T)⌝ ∨
+  ∃ a,
+    ⌜ga = TExp (TInt 0) [a]⌝ ∗
+    (public a ↔ ▷ □ session_fail si) ∗
+    (∀ t, dh_pred a t ↔ ▷ □ dh_auth_pred t)))%I
+  with "[hon_auth H3 H4]"
+  as "{p_m3} > [hon_auth #i_m3]".
+{ iDestruct "p_m3" as "[(p_skI & _) | (#i_m3 & _ & _)]".
+  { iMod (public_atI with "[//] H3 hon_auth p_skI")
+      as "[hon_auth #comp]" => //; try by solve_ndisj.
+    iPoseProof (honest_frag_public_at with "honR comp") as "%" => //.
+    iFrame. iLeft. iIntros "!> !>". iSplit.
+    - by iLeft.
+    - by iIntros "%"; tauto. }
+  iMod (lc_fupd_elim_later_pers with "H4 i_m3") as "{i_m3} #i_m3".
+  iDestruct "i_m3" as "(%a & %gb' & %kR' & %n' & %T' & %e_m3 &
+                        p_a & pred_a & honI & i_m3)".
+  case/Spec.of_list_inj: e_m3 => -> <- <- {ga gb' kR'} in gb gab kS si *.
+  iDestruct "i_m3" as "[i_m3 | i_m3]".
+  { iPoseProof (public_at_public with "i_m3") as "i_m3'".
+    iMod (public_atI with "[//] H3 hon_auth i_m3'")
+      as "[hon_auth #comp]" => //; try by solve_ndisj.
+    iPoseProof (honest_frag_public_at with "honR comp") as "%" => //.
+    iFrame. iLeft. iIntros "!> !>". iSplit.
+    - by iRight.
+    - by iIntros "%"; tauto. }
+  rewrite Spec.texpA TExpC2 -(Spec.texpA _ [a] b) -/gab -/kS.
+  iPoseProof (term_meta_agree with "info i_m3") as "{i_m3} %e".
+  case: e => <- {n'}.
+  iPoseProof (honest_frag_agree with "honR honI") as "->".
+  iModIntro. iFrame.
+  iRight. iModIntro. iExists a. by do ![iSplitL => //]. }
+iAssert (minted kS) as "#m_kS".
+{ iApply minted_tag.
+  rewrite minted_of_list /=. do !iSplit => //.
+  - by iApply public_minted.
+  - iApply minted_texp => //. }
+iAssert (minted kI) as "#m_kI".
+{ iApply minted_TKey. by iApply public_minted. }
+wp_pures. wp_bind (mkskey _). iApply wp_mkskey. wp_pures.
+iAssert (□ (∀ kt, public (TKey kt kS) ↔ ▷ session_fail si))%I
+  as "#sec_sk".
+{ iIntros "!> %kt". iSplit; last first.
+  { iIntros "#comp". iApply public_TKey. iLeft.
+    iApply public_tag.
+    rewrite public_of_list /=.
+    do !iSplit => //.
+    iApply public_texp => //.
+    iApply "p_b". eauto. }
+  iIntros "#p_sk".
+  iPoseProof (public_sym_keyE with "[//] p_sk") as ">p_kS".
+  iDestruct "i_m3" as "[[? compromise]|i_m3]" => //.
+  iDestruct "i_m3" as "(%a & -> & p_a & pred_a)".
+  rewrite Spec.texpA TExpC2 in gab kS si *.
+  rewrite public_of_list /=.
+  iDestruct "p_kS" as "(_ & _ & p_kS & _)".
+  rewrite /gab public_TExp2.
+  iDestruct "p_kS" as "[[_ p_b'] | [ [_ p_a'] | (_ & contra & _)]]".
+  - iPoseProof ("p_b" with "p_b'") as "?". by eauto.
+  - iPoseProof ("p_a" with "p_a'") as "{p_a} p_a". by eauto.
+  + iPoseProof ("pred_a" with "contra") as ">%contra".
+    by have := contra _ _ eq_refl. }
+iApply ("Hpost" $! (Some (TKey Dec kI, kS))).
+iFrame. iModIntro. iExists kI. by do !iSplit => //.
+Qed.
+
+End Verif.
