dh_auth/shared.v
@@ -1,0 +1,157 @@
+From stdpp Require Import base gmap.
+From mathcomp Require Import ssreflect.
+From mathcomp Require ssrbool.
+From iris.algebra Require Import agree auth csum gset gmap excl frac.
+From iris.algebra Require Import reservation_map.
+From iris.heap_lang Require Import notation proofmode.
+From cryptis Require Import lib term gmeta nown cryptis primitives tactics.
+From cryptis Require Import role.
+
+Set Implicit Arguments.
+Unset Strict Implicit.
+Unset Printing Implicit Defensive.
+
+Record sess_info := SessInfo {
+  si_init : term;
+  si_resp : term;
+  si_key  : term;
+  si_time : nat;
+  si_hon  : gset term;
+}.
+
+Global Instance sess_info_inhabited : Inhabited sess_info :=
+  populate (SessInfo inhabitant inhabitant inhabitant inhabitant inhabitant).
+
+Section Verif.
+
+Context `{!heapGS Σ, !cryptisGS Σ}.
+Notation iProp := (iProp Σ).
+
+Implicit Types (rl : role) (t kI kR nI nR sI sR kS : term).
+Implicit Types (γ γa γb : gname) (ok : bool).
+Implicit Types (ts : nat) (T : gset term).
+Implicit Types (si : sess_info).
+
+Variable N : namespace.
+
+(*
+
+A --> B: g^a; vkA
+B --> A: {g^a; g^b; vkA}@skB
+A --> B: {g^a; g^b; vkB}@skA
+
+g^{nAnB}
+
+*)
+
+Definition mkkeyshare : val := λ: "k",
+  texp (tgroup (tint #0)) "k".
+
+Lemma wp_mkkeyshare (t : term) E :
+  {{{ True }}}
+    mkkeyshare t @ E
+  {{{ RET (repr (TExp (TInt 0) [t])); True : iProp}}}.
+Proof.
+iIntros "%Φ _ Hpost". wp_lam.
+wp_bind (tint _). iApply wp_tint.
+wp_bind (tgroup _). iApply wp_tgroup.
+wp_bind (texp _ _). iApply wp_texp. rewrite Spec.texpA.
+by iApply "Hpost".
+Qed.
+
+Definition dh_auth_pred t : iProp :=
+  ⌜∀ g ks, t = TExp g ks → length ks = 1⌝.
+
+Definition session_fail si : iProp :=
+  public_at (si_time si) (TKey Enc (si_init si)) ∨
+  public_at (si_time si) (TKey Enc (si_resp si)).
+
+Definition session si : iProp :=
+  ◯H{si_time si} si_hon si ∗
+  term_meta (si_key si) (nroot.@"info")
+    (si_init si, si_resp si, si_time si).
+
+Lemma session_agree si1 si2 :
+  si_key si1 = si_key si2 →
+  session si1 -∗ session si2 -∗ ⌜si1 = si2⌝.
+Proof.
+case: si1 si2 => [kI1 kR1 kS n1 T1] [kI2 kR2 _ n2 T2] /= <-.
+iIntros "[#hon1 #meta1] [#hon2 #meta2] /=".
+iPoseProof (term_meta_agree with "meta1 meta2") as "%e".
+case: e => <- <- <-.
+by iPoseProof (honest_frag_agree with "hon1 hon2") as "->".
+Qed.
+
+Definition msg2_pred kR m2 : iProp :=
+  ∃ ga b kI n T,
+    let gb := TExp (TInt 0) [b] in
+    let gab := Spec.texp ga b in
+    let secret := Spec.of_list [ga; gb; gab] in
+    let kS := Spec.tag (nroot.@"keys".@"sym") secret in
+    ⌜m2 = Spec.of_list [ga; gb; TKey Dec kI]⌝ ∗
+    minted_at n ga ∗
+    (public b ↔ ▷ □ (public_at n (TKey Enc kI) ∨
+                     public_at n (TKey Enc kR))) ∗
+    (∀ t, dh_pred b t ↔ ▷ □ dh_auth_pred t) ∗
+    ◯H{n} T ∗
+    escrow cryptisN
+      (term_token ga ⊤)
+      (term_token kS (↑nroot.@"client")) ∗
+    term_meta kS (nroot.@"info") (kI, kR, n).
+
+Definition msg3_pred kI m3 : iProp :=
+  ∃ a gb kR n T,
+    let ga := TExp (TInt 0) [a] in
+    let gab := Spec.texp gb a in
+    let secret := Spec.of_list [ga; gb; gab] in
+    let kS := Spec.tag (nroot.@"keys".@"sym") secret in
+    ⌜m3 = Spec.of_list [ga; gb; TKey Dec kR]⌝ ∗
+    (public a ↔ ▷ □ (public_at n (TKey Enc kI) ∨
+                     public_at n (TKey Enc kR))) ∗
+    (∀ t, dh_pred a t ↔ ▷ □ dh_auth_pred t) ∗
+    ◯H{n} T ∗
+    (public_at n (TKey Enc kR) ∨ term_meta kS (nroot.@"info") (kI, kR, n)).
+
+Definition dh_auth_ctx : iProp :=
+  enc_pred (N.@"m2") msg2_pred ∗
+  enc_pred (N.@"m3") msg3_pred.
+
+Lemma dh_auth_ctx_alloc E :
+  ↑N ⊆ E →
+  enc_pred_token E ==∗
+  dh_auth_ctx.
+Proof.
+iIntros "%sub token".
+iMod (enc_pred_set (N.@"m2") msg2_pred with "token")
+  as "[#? token]"; try solve_ndisj.
+iMod (enc_pred_set (N.@"m3") msg3_pred with "token")
+  as "[#? token]"; try solve_ndisj.
+iModIntro. by iSplit.
+Qed.
+
+Section WithSSRBool.
+
+Import ssrbool.
+
+Lemma eq_texp2 g a1 a2 b1 b2 :
+  Spec.texp a1 b1 = Spec.texp (TExp g [a2]) b2 →
+  a1 = TExp g [a2] ∧ b1 = b2 ∨
+  a1 = TExp g [b2] ∧ b1 = a2.
+Proof.
+move=> e.
+have /Spec.is_expP [g' [] ks e_exp] : is_true (is_exp a1).
+  case exp: is_exp => //.
+  rewrite Spec.is_expN_texp // ?exp //= in e *; auto.
+  suff: is_true (is_exp (TInt 0)) by [].
+  by rewrite e Spec.texpA is_exp_TExp.
+rewrite {}e_exp !Spec.texpA {a1} in e *. symmetry in e.
+case/TExp_inj: e => <- {g'} /(@Permutation_length_2_inv _ _ _ _) [].
+- case=> <- -> {b2 ks}. by eauto.
+- case=> <- -> {a2 ks}. by eauto.
+Qed.
+
+End WithSSRBool.
+
+End Verif.
+
+Arguments dh_auth_ctx_alloc {Σ _ _} N E.
